Coq/Automaton/Automaton.v
@@ -1,0 +1,109 @@
+Require Coq.Lists.List.
+
+Import List.ListNotations.
+
+Local Open Scope list_scope.
+
+Require Export ZArith_base.
+
+Import BinIntDef.Z.
+
+Local Open Scope Z_scope.
+
+Inductive move : Type :=
+| Left
+| Right
+| Up
+| Down.
+
+Definition eq_dec (x y : move) : {x = y} + {x <> y}.
+Proof.
+ decide equality.
+Defined.
+
+
+Compute move_rect.
+
+Definition move_set := list move.
+
+Inductive base_state : Type :=
+  { x : Z;
+    y : Z;
+  }.
+
+Compute (x {| x := 3; y := 4 |}).
+
+
+(*  | 0,0 | 0,1 | 0,2  | 0,3  | 0,4   | 0,5 | *)
+(*  |-----+-----+------+------+-------+-----| *)
+(*  | 1,0 |     |      |      |       |     | *)
+(*  | 2,0 |     |      |  up  |       |     | *)
+(*  | 3,0 |     | left | here | right |     | *)
+(*  | 4,0 |     |      | down |       |     | *)
+(*  | 5,0 |     |      |      |       |     | *)
+Definition app_inst (s : base_state) (move : move) : base_state :=
+  match move with
+  | Left  => {|x := x s;     y := y s - 1|}
+  | Right => {|x := x s;     y := y s + 1|}
+  | Up    => {|x := x s - 1; y := y s|}
+  | Down  => {|x := x s + 1; y := y s|}
+  end.
+
+Definition run (s : base_state) (moves : move_set) := List.fold_left app_inst moves s.
+
+Compute (List.count_occ Z.eq_dec [2;3;4] 3).
+
+Compute Z.eqb.
+
+Definition left  (xs : move_set) : nat := List.count_occ eq_dec xs Left.
+Definition right (xs : move_set) : nat := List.count_occ eq_dec xs Right.
+Definition up    (xs : move_set) : nat := List.count_occ eq_dec xs Up.
+Definition down  (xs : move_set) : nat := List.count_occ eq_dec xs Down.
+
+Definition default_spot := {| x := 0; y := 0|}.
+
+
+
+
+(* prove the more general case first *)
+(* Lemma x_bounded : forall (moves : move_set) (state : base_state), *)
+(*     left moves = right moves -> y state = y (run state moves). *)
+(* Proof. *)
+(*   intros m . *)
+(*   induction m as [| m' IHm']. *)
+(*   - simpl. *)
+(*     reflexivity. *)
+(*   - intros s impl. *)
+(*     destruct m' eqn:E. *)
+(*     (* Figure out how to remove this repeat call!!! *) *)
+(*     (* Also simplify this proof... kind of a mess of unfodling *) *)
+(*     Focus 3. *)
+(*     simpl; *)
+(*     unfold left in impl; *)
+(*     unfold right in impl; *)
+(*     simpl in impl; *)
+(*     unfold left in IHIHm'; *)
+(*     unfold right in IHIHm'; *)
+(*     rewrite <- impl in IHIHm'; *)
+(*     simpl in IHIHm'; *)
+(*     rewrite <- IHIHm' at 1; *)
+(*     reflexivity. *)
+(*     (* Figure out how to remove this repeat call!!! *) *)
+(*     Focus 3. *)
+(*     simpl; *)
+(*     unfold left in impl; *)
+(*     unfold right in impl; *)
+(*     simpl in impl; *)
+(*     unfold left in IHIHm'; *)
+(*     unfold right in IHIHm'; *)
+(*     rewrite <- impl in IHIHm'; *)
+(*     simpl in IHIHm'; *)
+(*     rewrite <- IHIHm' at 1; *)
+(*     reflexivity. *)
+(*     + unfold left in impl. *)
+(*       unfold right in impl. *)
+(*       simpl in impl. *)
+(*       unfold left in IHIHm'. *)
+(*       unfold right in IHIHm'. *)
+(* admit. *)
+
