Fstar/fun/Automaton/Automaton.fst
@@ -1,0 +1,119 @@
+module Automaton
+
+module List = FStar.List.Tot
+open FStar.Tactics
+open FStar.Tactics.Derived
+
+(**** four move machine *)
+
+type move =
+  | Left
+  | Right
+  | Up
+  | Down
+
+type move_set = list move
+
+(* Useful for the turning machine, when we look in a direction *)
+type direction = move
+val direction_to_mod_4 : move -> n : nat{n < 4}
+let direction_to_mod_4 = function
+  | Left  -> 0
+  | Right -> 2
+  | Up    -> 1
+  | Down  -> 3
+
+
+type base_state = {
+  spot : int * int
+}
+
+
+// | 0,0 | 0,1 | 0,2  | 0,3  | 0,4   | 0,5 |
+// |-----+-----+------+------+-------+-----|
+// | 1,0 |     |      |      |       |     |
+// | 2,0 |     |      |  up  |       |     |
+// | 3,0 |     | left | here | right |     |
+// | 4,0 |     |      | down |       |     |
+// | 5,0 |     |      |      |       |     |
+
+val app_inst : base_state -> move -> base_state
+let app_inst {spot} move =
+  let (x,y) = spot in
+  { spot =
+      match move with
+      | Left  -> (x    , y - 1)
+      | Right -> (x    , y + 1)
+      | Up    -> (x - 1, y)
+      | Down  -> (x + 1, y)
+  }
+
+
+val run : base_state -> move_set -> base_state
+let run s xs = List.fold_left app_inst s xs
+
+let left  = List.count Left
+let right = List.count Right
+let up    = List.count Up
+let down  = List.count Down
+
+
+val run_n_times : n : nat -> base_state -> move_set -> base_state
+let rec run_n_times n s xs =
+  match n with
+  | 0 -> s
+  | n -> run_n_times (n - 1) (run s xs) xs
+
+let default_spot = {spot = (0,0)}
+
+let spot_to_int {spot} = let (x,y) = spot in x + y
+
+
+let test = run default_spot [Left; Right; Up; Down]
+
+
+(* TODO ∷ learn to abstract this logic into 1 call, via tactitcs? *)
+
+val y_relationship : xs : move_set
+                   → s  : base_state
+                   → Lemma (snd s.spot + (right xs - left xs) == (snd (run s xs).spot))
+let rec y_relationship xs s =
+  match xs with
+  | []         -> ()
+  | Up    :: xs -> y_relationship xs (app_inst s Up)
+  | Down  :: xs -> y_relationship xs (app_inst s Down)
+  | Left  :: xs -> y_relationship xs (app_inst s Left)
+  | Right :: xs -> y_relationship xs (app_inst s Right)
+
+
+val x_relationship : xs : move_set
+                   → s  : base_state
+                   → Lemma (fst s.spot + (down xs - up xs) == (fst (run s xs).spot))
+let rec x_relationship xs s =
+  match xs with
+  | []         -> ()
+  | Up    :: xs -> x_relationship xs (app_inst s Up)
+  | Down  :: xs -> x_relationship xs (app_inst s Down)
+  | Left  :: xs -> x_relationship xs (app_inst s Left)
+  | Right :: xs -> x_relationship xs (app_inst s Right)
+
+val proof_bounded : xs  : move_set
+                  -> spot : base_state
+                  → Lemma (requires left xs == right xs /\ up xs == down xs)
+                          (ensures spot == run spot xs)
+let proof_bounded xs state =
+  x_relationship xs state;
+  y_relationship xs state
+
+
+val proof_bounded_n : xs   : move_set
+                    → spot : base_state
+                    → n    : nat
+                    → Lemma (requires left xs == right xs /\ up xs == down xs)
+                            (ensures spot == run_n_times n spot xs)
+let rec proof_bounded_n xs spot n =
+  match n with
+  | 0 -> ()
+  | n ->
+    proof_bounded xs spot;
+    proof_bounded_n xs spot (n - 1)
